semantic invariants

theories/base_logic/lib/invariants.v
@@ -6,40 +6,6 @@ From iris.base_logic.lib Require Import wsat.
 Set Default Proof Using "Type".
 Import uPred.
 
-(** Derived forms and lemmas about them. *)
-Definition inv_def `{!invG Σ} (N : namespace) (P : iProp Σ) : iProp Σ :=
-  (∃ i P', ⌜i ∈ (↑N:coPset)⌝ ∧ ▷ □ (P' ↔ P) ∧ ownI i P')%I.
-Definition inv_aux : seal (@inv_def). by eexists. Qed.
-Definition inv {Σ i} := inv_aux.(unseal) Σ i.
-Definition inv_eq : @inv = @inv_def := inv_aux.(seal_eq).
-Instance: Params (@inv) 3 := {}.
-Typeclasses Opaque inv.
-
-Section inv.
-Context `{!invG Σ}.
-Implicit Types i : positive.
-Implicit Types N : namespace.
-Implicit Types P Q R : iProp Σ.
-
-Global Instance inv_contractive N : Contractive (inv N).
-Proof. rewrite inv_eq. solve_contractive. Qed.
-
-Global Instance inv_ne N : NonExpansive (inv N).
-Proof. apply contractive_ne, _. Qed.
-
-Global Instance inv_proper N : Proper ((⊣⊢) ==> (⊣⊢)) (inv N).
-Proof. apply ne_proper, _. Qed.
-
-Global Instance inv_persistent N P : Persistent (inv N P).
-Proof. rewrite inv_eq /inv; apply _. Qed.
-
-Lemma inv_iff N P Q : ▷ □ (P ↔ Q) -∗ inv N P -∗ inv N Q.
-Proof.
-  iIntros "#HPQ". rewrite inv_eq. iDestruct 1 as (i P') "(?&#HP&?)".
-  iExists i, P'. iFrame. iNext; iAlways; iSplit.
-  - iIntros "HP'". iApply "HPQ". by iApply "HP".
-  - iIntros "HQ". iApply "HP". by iApply "HPQ".
-Qed.
 
 Lemma fresh_inv_name (E : gset positive) N : ∃ i, i ∉ E ∧ i ∈ (↑N:coPset).
 Proof.
@@ -50,79 +16,179 @@ Proof.
   apply gset_to_coPset_finite.
 Qed.
 
-Lemma inv_alloc N E P : ▷ P ={E}=∗ inv N P.
-Proof.
-  rewrite inv_eq /inv_def uPred_fupd_eq. iIntros "HP [Hw $]".
-  iMod (ownI_alloc (.∈ (↑N : coPset)) P with "[$HP $Hw]")
-    as (i ?) "[$ ?]"; auto using fresh_inv_name.
-  do 2 iModIntro. iExists i, P. rewrite -(iff_refl True%I). auto.
-Qed.
+(** * Invariants *)
+Section inv.
+  Context `{!invG Σ}.
 
-Lemma inv_alloc_open N E P :
-  ↑N ⊆ E → (|={E, E∖↑N}=> inv N P ∗ (▷P ={E∖↑N, E}=∗ True))%I.
-Proof.
-  rewrite inv_eq /inv_def uPred_fupd_eq. iIntros (Sub) "[Hw HE]".
-  iMod (ownI_alloc_open (.∈ (↑N : coPset)) P with "Hw")
-    as (i ?) "(Hw & #Hi & HD)"; auto using fresh_inv_name.
-  iAssert (ownE {[i]} ∗ ownE (↑ N ∖ {[i]}) ∗ ownE (E ∖ ↑ N))%I
-    with "[HE]" as "(HEi & HEN\i & HE\N)".
-  { rewrite -?ownE_op; [|set_solver..].
-    rewrite assoc_L -!union_difference_L //. set_solver. }
-  do 2 iModIntro. iFrame "HE\N". iSplitL "Hw HEi"; first by iApply "Hw".
-  iSplitL "Hi".
-  { iExists i, P. rewrite -(iff_refl True%I). auto. }
-  iIntros "HP [Hw HE\N]".
-  iDestruct (ownI_close with "[$Hw $Hi $HP $HD]") as "[$ HEi]".
-  do 2 iModIntro. iSplitL; [|done].
-  iCombine "HEi HEN\i HE\N" as "HEN".
-  rewrite -?ownE_op; [|set_solver..].
-  rewrite assoc_L -!union_difference_L //; set_solver.
-Qed.
+  (** Internal backing store of invariants *)
+  Definition internal_inv_def (N : namespace) (P : iProp Σ) : iProp Σ :=
+    (∃ i P', ⌜i ∈ (↑N:coPset)⌝ ∧ ▷ □ (P' ↔ P) ∧ ownI i P')%I.
+  Definition internal_inv_aux : seal (@internal_inv_def). by eexists. Qed.
+  Definition internal_inv := internal_inv_aux.(unseal).
+  Definition internal_inv_eq : @internal_inv = @internal_inv_def := internal_inv_aux.(seal_eq).
+  Typeclasses Opaque internal_inv.
 
-Lemma inv_open E N P :
-  ↑N ⊆ E → inv N P ={E,E∖↑N}=∗ ▷ P ∗ (▷ P ={E∖↑N,E}=∗ True).
-Proof.
-  rewrite inv_eq /inv_def uPred_fupd_eq /uPred_fupd_def.
-  iDestruct 1 as (i P') "(Hi & #HP' & #HiP)".
-  iDestruct "Hi" as % ?%elem_of_subseteq_singleton.
-  rewrite {1 4}(union_difference_L (↑ N) E) // ownE_op; last set_solver.
-  rewrite {1 5}(union_difference_L {[ i ]} (↑ N)) // ownE_op; last set_solver.
-  iIntros "(Hw & [HE $] & $) !> !>".
-  iDestruct (ownI_open i with "[$Hw $HE $HiP]") as "($ & HP & HD)".
-  iDestruct ("HP'" with "HP") as "$".
-  iIntros "HP [Hw $] !> !>". iApply (ownI_close _ P'). iFrame "HD Hw HiP".
-  iApply "HP'". iFrame.
-Qed.
+  Global Instance internal_inv_persistent N P : Persistent (internal_inv N P).
+  Proof. rewrite internal_inv_eq /internal_inv; apply _. Qed.
 
-Lemma inv_open_strong E N P :
-  ↑N ⊆ E → inv N P ={E,E∖↑N}=∗ ▷ P ∗ ∀ E', ▷ P ={E',↑N ∪ E'}=∗ True.
-Proof.
-  iIntros (?) "Hinv".
-  iPoseProof (inv_open (↑ N) N P with "Hinv") as "H"; first done.
-  rewrite difference_diag_L.
-  iPoseProof (fupd_mask_frame_r _ _ (E ∖ ↑ N) with "H") as "H"; first set_solver.
-  rewrite left_id_L -union_difference_L //. iMod "H" as "[$ H]"; iModIntro.
-  iIntros (E') "HP".
-  iPoseProof (fupd_mask_frame_r _ _ E' with "(H HP)") as "H"; first set_solver.
-  by rewrite left_id_L.
-Qed.
+  Lemma internal_inv_open E N P :
+  ↑N ⊆ E → internal_inv N P ={E,E∖↑N}=∗ ▷ P ∗ (▷ P ={E∖↑N,E}=∗ True).
+  Proof.
+    rewrite internal_inv_eq /internal_inv_def uPred_fupd_eq /uPred_fupd_def.
+    iDestruct 1 as (i P') "(Hi & #HP' & #HiP)".
+    iDestruct "Hi" as % ?%elem_of_subseteq_singleton.
+    rewrite {1 4}(union_difference_L (↑ N) E) // ownE_op; last set_solver.
+    rewrite {1 5}(union_difference_L {[ i ]} (↑ N)) // ownE_op; last set_solver.
+    iIntros "(Hw & [HE $] & $) !> !>".
+    iDestruct (ownI_open i with "[$Hw $HE $HiP]") as "($ & HP & HD)".
+    iDestruct ("HP'" with "HP") as "$".
+    iIntros "HP [Hw $] !> !>". iApply (ownI_close _ P'). iFrame "HD Hw HiP".
+    iApply "HP'". iFrame.
+  Qed.
 
-Global Instance into_inv_inv N P : IntoInv (inv N P) N := {}.
+  Lemma internal_inv_alloc N E P : ▷ P ={E}=∗ internal_inv N P.
+  Proof.
+    rewrite internal_inv_eq /internal_inv_def uPred_fupd_eq. iIntros "HP [Hw $]".
+    iMod (ownI_alloc (.∈ (↑N : coPset)) P with "[$HP $Hw]")
+      as (i ?) "[$ ?]"; auto using fresh_inv_name.
+    do 2 iModIntro. iExists i, P. rewrite -(iff_refl True%I). auto.
+  Qed.
 
-Global Instance into_acc_inv E N P :
-  IntoAcc (X:=unit) (inv N P) 
-          (↑N ⊆ E) True (fupd E (E∖↑N)) (fupd (E∖↑N) E)
-          (λ _, ▷ P)%I (λ _, ▷ P)%I (λ _, None)%I.
-Proof.
-  rewrite /IntoAcc /accessor exist_unit.
-  iIntros (?) "#Hinv _". iApply inv_open; done.
-Qed.
+  Lemma internal_inv_alloc_open N E P :
+    ↑N ⊆ E → (|={E, E∖↑N}=> internal_inv N P ∗ (▷P ={E∖↑N, E}=∗ True))%I.
+  Proof.
+    rewrite internal_inv_eq /internal_inv_def uPred_fupd_eq. iIntros (Sub) "[Hw HE]".
+    iMod (ownI_alloc_open (.∈ (↑N : coPset)) P with "Hw")
+      as (i ?) "(Hw & #Hi & HD)"; auto using fresh_inv_name.
+    iAssert (ownE {[i]} ∗ ownE (↑ N ∖ {[i]}) ∗ ownE (E ∖ ↑ N))%I
+      with "[HE]" as "(HEi & HEN\i & HE\N)".
+    { rewrite -?ownE_op; [|set_solver..].
+      rewrite assoc_L -!union_difference_L //. set_solver. }
+    do 2 iModIntro. iFrame "HE\N". iSplitL "Hw HEi"; first by iApply "Hw".
+    iSplitL "Hi".
+    { iExists i, P. rewrite -(iff_refl True%I). auto. }
+    iIntros "HP [Hw HE\N]".
+    iDestruct (ownI_close with "[$Hw $Hi $HP $HD]") as "[$ HEi]".
+    do 2 iModIntro. iSplitL; [|done].
+    iCombine "HEi HEN\i HE\N" as "HEN".
+    rewrite -?ownE_op; [|set_solver..].
+    rewrite assoc_L -!union_difference_L //; set_solver.
+  Qed.
 
-Lemma inv_open_timeless E N P `{!Timeless P} :
-  ↑N ⊆ E → inv N P ={E,E∖↑N}=∗ P ∗ (P ={E∖↑N,E}=∗ True).
-Proof.
-  iIntros (?) "Hinv". iMod (inv_open with "Hinv") as "[>HP Hclose]"; auto.
-  iIntros "!> {$HP} HP". iApply "Hclose"; auto.
-Qed.
+  (** Invariants API *)
+  Definition inv_def (N: namespace) (P: iProp Σ) : iProp Σ :=
+    (□ (∀ E, ⌜↑N ⊆ E⌝ → |={E,E ∖ ↑N}=> ▷ P ∗ (▷ P ={E ∖ ↑N,E}=∗ True)))%I.
+  Definition inv_aux : seal (@inv_def). by eexists. Qed.
+  Definition inv := inv_aux.(unseal).
+  Definition inv_eq : @inv = @inv_def := inv_aux.(seal_eq).
+  Typeclasses Opaque inv.
+
+  (** Properties about invariants *)
+  Global Instance inv_contractive N: Contractive (inv N).
+  Proof. rewrite inv_eq. solve_contractive. Qed.
+
+  Global Instance inv_ne N : NonExpansive (inv N).
+  Proof. apply contractive_ne, _. Qed.
+
+  Global Instance inv_proper N: Proper (equiv ==> equiv) (inv N).
+  Proof. apply ne_proper, _. Qed.
+
+  Global Instance inv_persistent M P: Persistent (inv M P).
+  Proof. rewrite inv_eq. typeclasses eauto. Qed.
+
+  Lemma inv_acc N P Q:
+    inv N P -∗ ▷ □ (P -∗ Q ∗ (Q -∗ P)) -∗ inv N Q.
+  Proof.
+    iIntros "#I #Acc". rewrite inv_eq.
+    iModIntro. iIntros (E H). iDestruct ("I" $! E H) as "#I'".
+    iApply fupd_wand_r. iFrame "I'".
+    iIntros "(P & Hclose)". iSpecialize ("Acc" with "P").
+    iDestruct "Acc" as "[Q CB]". iFrame.
+    iIntros "Q". iApply "Hclose". now iApply "CB".
+  Qed.
+
+  Lemma inv_iff N P Q : ▷ □ (P ↔ Q) -∗ inv N P -∗ inv N Q.
+  Proof.
+    iIntros "#HPQ #I". iApply (inv_acc with "I").
+    iNext. iIntros "!# P". iSplitL "P".
+    - by iApply "HPQ".
+    - iIntros "Q". by iApply "HPQ".
+  Qed.
+
+  Lemma inv_to_inv M P: internal_inv M P  -∗ inv M P.
+  Proof.
+    iIntros "#I". rewrite inv_eq. iIntros (E H).
+    iPoseProof (internal_inv_open with "I") as "H"; eauto.
+  Qed.
+
+  Lemma inv_alloc N E P : ▷ P ={E}=∗ inv N P.
+  Proof.
+    iIntros "P". iPoseProof (internal_inv_alloc  N E with "P") as "I".
+    iApply fupd_mono; last eauto.
+    iApply inv_to_inv.
+  Qed.
+
+  Lemma inv_alloc_open N E P :
+    ↑N ⊆ E → (|={E, E∖↑N}=> inv N P ∗ (▷P ={E∖↑N, E}=∗ True))%I.
+  Proof.
+    iIntros (H). iPoseProof (internal_inv_alloc_open _ _ _ H) as "H".
+    iApply fupd_mono; last eauto.
+    iIntros "[I H]"; iFrame; by iApply inv_to_inv.
+  Qed.
+
+  Lemma inv_open E N P :
+    ↑N ⊆ E → inv N P ={E,E∖↑N}=∗ ▷ P ∗ (▷ P ={E∖↑N,E}=∗ True).
+  Proof.
+    rewrite inv_eq /inv_def; iIntros (H) "#I". by iApply "I".
+  Qed.
+
+  Lemma inv_open_strong E N P :
+    ↑N ⊆ E → inv N P ={E,E∖↑N}=∗ ▷ P ∗ ∀ E', ▷ P ={E',↑N ∪ E'}=∗ True.
+  Proof.
+      iIntros (?) "Hinv".      iPoseProof (inv_open (↑ N) N P with "Hinv") as "H"; first done.
+      rewrite difference_diag_L.
+      iPoseProof (fupd_mask_frame_r _ _ (E ∖ ↑ N) with "H") as "H"; first set_solver.
+      rewrite left_id_L -union_difference_L //. iMod "H" as "[$ H]"; iModIntro.
+      iIntros (E') "HP".
+      iPoseProof (fupd_mask_frame_r _ _ E' with "(H HP)") as "H"; first set_solver.
+        by rewrite left_id_L.
+  Qed.
+
+  Global Instance into_inv_inv N P : IntoInv (inv N P) N := {}.
+
+  Global Instance into_acc_inv N P E:
+    IntoAcc (X := unit) (inv N P)
+            (↑N ⊆ E) True (fupd E (E ∖ ↑N)) (fupd (E ∖ ↑N) E)
+            (λ _ : (), (▷ P)%I) (λ _ : (), (▷ P)%I) (λ _ : (), None).
+  Proof.
+    rewrite inv_eq /IntoAcc /accessor bi.exist_unit.
+    iIntros (?) "#Hinv _". iApply "Hinv"; done.
+  Qed.
+
+  Lemma inv_open_timeless E N P `{!Timeless P} :
+    ↑N ⊆ E → inv N P ={E,E∖↑N}=∗ P ∗ (P ={E∖↑N,E}=∗ True).
+  Proof.
+    iIntros (?) "Hinv". iMod (inv_open with "Hinv") as "[>HP Hclose]"; auto.
+    iIntros "!> {$HP} HP". iApply "Hclose"; auto.
+  Qed.
+
+  (* Weakening of semantic invariants *)
+  Lemma inv_proj_l N P Q: inv N (P ∗ Q) -∗ inv N P.
+  Proof.
+    iIntros "#I". iApply inv_acc; eauto.
+    iNext. iIntros "!# [$ Q] P"; iFrame.
+  Qed.
+
+  Lemma inv_proj_r N P Q: inv N (P ∗ Q) -∗ inv N Q.
+  Proof.
+    rewrite (bi.sep_comm P Q). eapply inv_proj_l.
+  Qed.
+
+  Lemma inv_split N P Q: inv N (P ∗ Q) -∗ inv N P ∗ inv N Q.
+  Proof.
+    iIntros "#H".
+    iPoseProof (inv_proj_l with "H") as "$".
+    iPoseProof (inv_proj_r with "H") as "$".
+  Qed.
 
 End inv.
